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Curvature and Shear Vorticity in Cartesian Coordinates 
 

Sharan Majumdar, 6/10/20.  Using Bleck (JAS, 1991)1 
 
Cartesian Coordinates 

𝒙 = 𝑥	𝒊 + 𝑦	𝒋 + 𝑧	𝒌 = (𝑥, 𝑦, 𝑧) 
Horizontal Velocity 

𝒗 = 𝑢	𝒊 + 𝑣	𝒋 = (𝑢, 𝑣, 0)	 
Relative Vorticity 

𝜁 = 	𝒌 ∙ (𝛻 × 𝒗) = 	
𝜕𝑣
𝜕𝑥 −	

𝜕𝑢
𝜕𝑦	

Natural Coordinates 
 
Unit tangent vector 

𝒕 = 	
1

√𝑢! +	𝑣!
	𝒗 = 	

𝒗
𝑉 

Unit normal vector	
𝒏 = 𝒌	 × 	𝒕 

Velocity 
𝒗 = 𝑉	𝒕 

Relative Vorticity 

𝜁 = 	−	
𝜕𝑉
𝜕𝑛 +	

𝑉
𝑅"

 

			= 	 						𝜁# 	+ 	𝜁" 	
= Shear	vorticity + Curvature	Vorticity 

 
Calculus Identities for below 

𝜕
𝜕𝑛 	≡ 𝒏	 ∙ 	∇ 

∇ × (𝐴𝒃) 	≡ 𝐴	∇ × 𝒃 + (∇A) × 𝒃	
𝒂 ∙ (𝒃 × 𝒄) ≡ −𝒃 ∙ (𝒂 × 𝒄) 

 
Rewrite relative vorticity as 

𝜁 = 	𝒌 ∙ (𝛻 × 𝑉𝒕)	
Shear vorticity 

𝜁# =	−	
𝜕𝑉
𝜕𝑛 = −𝒏	 ∙ 	∇𝑉 = 	−∇𝑉 ∙ 𝒏 

=	−∇𝑉 ∙ (𝒌 × 𝒕) 
= 	𝒌 ∙ (∇𝑉 × 𝒕) 

 
We use this to reformulate the curvature vorticity (on next page): 

 
1 https://journals.ametsoc.org/jas/article/48/8/1124/22892/Tendency-Equations-for-Shear-and-Curvature  
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	𝜁" = 	𝜁 −	𝜁# 
= 	𝒌 ∙ (𝛻 × 𝑉𝒕) − 	𝒌 ∙ (∇𝑉 × 𝒕)	
= 𝑉	𝒌 ∙ (𝛻 × 𝒕)	

= 𝑉	𝒌 ∙ T𝛻 × U
1

√𝑢! +	𝑣!
	𝒗VW	

= 𝑉	𝒌 ∙ TU
1

√𝑢! +	𝑣!
	𝛻 × 𝒗V+	𝛻 U

1
√𝑢! +	𝑣!

V × 𝒗W	

= 	𝜁 + 	𝑉𝒌 ∙ T𝛻 U
1

√𝑢! +	𝑣!
V × 𝒗W	

= 	𝜁 + 	𝑉𝒌 ∙ T−
1
𝑉$ U𝑢

𝜕𝑢
𝜕𝑥 + 𝑣	

𝜕𝑣
𝜕𝑥 , 𝑢

𝜕𝑢
𝜕𝑦 + 𝑣	

𝜕𝑣
𝜕𝑦V × 𝒗W	

= 	𝜁 −
1
𝑉! U𝑣𝑢

𝜕𝑢
𝜕𝑥 + 𝑣𝑣

𝜕𝑣
𝜕𝑥 − 𝑢𝑢

𝜕𝑢
𝜕𝑦 − 𝑢𝑣

𝜕𝑣
𝜕𝑦V	

= 	𝜁 −
1
𝑉! (𝑢	𝑣)

⎝

⎜
⎛
𝜕𝑢
𝜕𝑥

𝜕𝑢
𝜕𝑦

𝜕𝑣
𝜕𝑥

𝜕𝑣
𝜕𝑦⎠

⎟
⎞
^
𝑣
−𝑢_ 

Hence, the shear vorticity	

𝜁# =
1
𝑉! U𝑣𝑢

𝜕𝑢
𝜕𝑥 + 𝑣𝑣

𝜕𝑣
𝜕𝑥 − 𝑢𝑢

𝜕𝑢
𝜕𝑦 − 𝑢𝑣

𝜕𝑣
𝜕𝑦V	

=
1
𝑉!
(𝑢	𝑣)

⎝

⎜
⎛
𝜕𝑢
𝜕𝑥

𝜕𝑢
𝜕𝑦

𝜕𝑣
𝜕𝑥

𝜕𝑣
𝜕𝑦⎠

⎟
⎞
^
𝑣
−𝑢_ 

Continuing with the curvature vorticity: 

𝜁" = 	𝜁 −
1
𝑉! U𝑣𝑢

𝜕𝑢
𝜕𝑥 + 𝑣𝑣

𝜕𝑣
𝜕𝑥 − 𝑢𝑢

𝜕𝑢
𝜕𝑦 − 𝑢𝑣

𝜕𝑣
𝜕𝑦V	

=
1
𝑉!
(𝑢𝑢 + 𝑣𝑣) U

𝜕𝑣
𝜕𝑥 −

𝜕𝑢
𝜕𝑦V −

1
𝑉! U𝑣𝑢

𝜕𝑢
𝜕𝑥 + 𝑣𝑣

𝜕𝑣
𝜕𝑥 − 𝑢𝑢

𝜕𝑢
𝜕𝑦 − 𝑢𝑣

𝜕𝑣
𝜕𝑦V 

Hence, the curvature vorticity 

𝜁" =
1
𝑉! U𝑢𝑢

𝜕𝑣
𝜕𝑥 − 𝑣𝑣

𝜕𝑢
𝜕𝑦 − 𝑣𝑢

𝜕𝑢
𝜕𝑥 + 𝑢𝑣

𝜕𝑣
𝜕𝑦V 

=
1
𝑉! (−𝑣	𝑢)

⎝

⎜
⎛
𝜕𝑢
𝜕𝑥

𝜕𝑢
𝜕𝑦

𝜕𝑣
𝜕𝑥

𝜕𝑣
𝜕𝑦⎠

⎟
⎞
^
𝑢
𝑣_ 

Adding the shear vorticity and curvature vorticity: 

𝜁# +	𝜁" =
1
𝑉! U𝑣𝑢

𝜕𝑢
𝜕𝑥 + 𝑣𝑣

𝜕𝑣
𝜕𝑥 − 𝑢𝑢

𝜕𝑢
𝜕𝑦 − 𝑢𝑣

𝜕𝑣
𝜕𝑦 + 𝑢𝑢

𝜕𝑣
𝜕𝑥 − 𝑣𝑣

𝜕𝑢
𝜕𝑦 − 𝑣𝑢

𝜕𝑢
𝜕𝑥 + 𝑢𝑣

𝜕𝑣
𝜕𝑦V	

=
1
𝑉! (𝑢

! + 𝑣!) U
𝜕𝑣
𝜕𝑥 −

𝜕𝑢
𝜕𝑦V = 	𝜁 


